scripts/fixtures/PrimitiveConversion.v
@@ -1,0 +1,87 @@
+From Stdlib Require Import ZArith List Floats Uint63.
+From Flocq Require Import IEEE754.PrimFloat IEEE754.BinarySingleNaN.
+Import ListNotations.
+Open Scope Z_scope.
+
+Definition inputs : list SpecFloat.spec_float :=
+  [SpecFloat.S754_finite false 3 (-1);
+   SpecFloat.S754_finite false 9223372036854775808 (0);
+   SpecFloat.S754_finite false 9223372036854775809 (0);
+   SpecFloat.S754_finite false 9223372036854775807 (0);
+   SpecFloat.S754_finite false 9007199254740997 (-1077);
+   SpecFloat.S754_zero false;
+   SpecFloat.S754_infinity false;
+   SpecFloat.S754_finite false 4503599627370496 (-52);
+   SpecFloat.S754_finite false 1 (-1074);
+   SpecFloat.S754_finite false 9007199254740991 (971);
+   SpecFloat.S754_finite false 1 (-1075);
+   SpecFloat.S754_finite false 3 (-1075);
+   SpecFloat.S754_finite false 1 (1024);
+   SpecFloat.S754_finite false 1 (-1000000000000000000000000000000);
+   SpecFloat.S754_finite false 1 (1000000000000000000000000000000);
+   SpecFloat.S754_finite true 3 (-1);
+   SpecFloat.S754_finite true 9223372036854775808 (0);
+   SpecFloat.S754_finite true 9223372036854775809 (0);
+   SpecFloat.S754_finite true 9223372036854775807 (0);
+   SpecFloat.S754_finite true 9007199254740997 (-1077);
+   SpecFloat.S754_zero true;
+   SpecFloat.S754_infinity true;
+   SpecFloat.S754_finite true 4503599627370496 (-52);
+   SpecFloat.S754_finite true 1 (-1074);
+   SpecFloat.S754_finite true 9007199254740991 (971);
+   SpecFloat.S754_finite true 1 (-1075);
+   SpecFloat.S754_finite true 3 (-1075);
+   SpecFloat.S754_finite true 1 (1024);
+   SpecFloat.S754_finite true 1 (-1000000000000000000000000000000);
+   SpecFloat.S754_finite true 1 (1000000000000000000000000000000);
+   SpecFloat.S754_nan].
+
+Definition expected : list SpecFloat.spec_float :=
+  [SpecFloat.S754_finite false 6755399441055744 (-52);
+   SpecFloat.S754_zero false;
+   SpecFloat.S754_finite false 4503599627370496 (-52);
+   SpecFloat.S754_finite false 4503599627370496 (11);
+   SpecFloat.S754_finite false 1125899906842624 (-1074);
+   SpecFloat.S754_zero false;
+   SpecFloat.S754_infinity false;
+   SpecFloat.S754_finite false 4503599627370496 (-52);
+   SpecFloat.S754_finite false 1 (-1074);
+   SpecFloat.S754_finite false 9007199254740991 (971);
+   SpecFloat.S754_zero false;
+   SpecFloat.S754_finite false 2 (-1074);
+   SpecFloat.S754_infinity false;
+   SpecFloat.S754_zero false;
+   SpecFloat.S754_infinity false;
+   SpecFloat.S754_finite true 6755399441055744 (-52);
+   SpecFloat.S754_zero true;
+   SpecFloat.S754_finite true 4503599627370496 (-52);
+   SpecFloat.S754_finite true 4503599627370496 (11);
+   SpecFloat.S754_finite true 1125899906842624 (-1074);
+   SpecFloat.S754_zero true;
+   SpecFloat.S754_infinity true;
+   SpecFloat.S754_finite true 4503599627370496 (-52);
+   SpecFloat.S754_finite true 1 (-1074);
+   SpecFloat.S754_finite true 9007199254740991 (971);
+   SpecFloat.S754_zero true;
+   SpecFloat.S754_finite true 2 (-1074);
+   SpecFloat.S754_infinity true;
+   SpecFloat.S754_zero true;
+   SpecFloat.S754_infinity true;
+   SpecFloat.S754_nan].
+
+Definition outputs := map (fun x => FloatOps.Prim2SF (FloatOps.SF2Prim x)) inputs.
+Example literal_conversions : outputs = expected.
+Proof. vm_compute. reflexivity. Qed.
+
+Example numeric_conversion_is_not_validation :
+    FloatOps.Prim2SF (FloatOps.SF2Prim (SpecFloat.S754_finite false 3 (-1))) <>
+      @BinarySingleNaN.B2SF 53 1024
+        (@BinarySingleNaN.SF2B' 53 1024 (SpecFloat.S754_finite false 3 (-1))).
+Proof. vm_compute. discriminate. Qed.
+
+Example two_roundings_are_not_one :
+    FloatOps.Prim2SF (FloatOps.SF2Prim (SpecFloat.S754_finite false 9007199254740997 (-1077))) =
+      SpecFloat.S754_finite false 1125899906842624 (-1074) /\
+    SpecFloat.binary_normalize 53 1024 9007199254740997 (-1077) false =
+      SpecFloat.S754_finite false 1125899906842625 (-1074).
+Proof. vm_compute. split; reflexivity. Qed.
